Compatible.v
@@ -1,6 +1,4 @@
-Require Import DataTypes.
-Require Import Channel.
-Require Import Cache.
+Require Import DataTypes Channel Cache.
 
 Module Type CompatBehavior (dt: DataTypes) (ch: ChannelPerAddr dt).
   Import dt ch.
@@ -8,45 +6,58 @@ Module Type CompatBehavior (dt: DataTypes) (ch: ChannelPerAddr dt).
     Context {n: Cache}.
     Context {a: Addr}.
     Context {t: Time}.
-    Axiom sendPCond: forall {p}, parent n p ->
+    Axiom sendPCond: forall {p}, defined n -> defined p -> parent n p ->
                                  forall {m},
                                    mark mch n p a t m ->
-                                   forall {c}, parent c n -> sle (dir n c a t) (to m).
-    Axiom sendCCond: forall {c},
+                                   forall {c}, defined c -> parent c n ->
+                                               sle (dir n c a t) (to m).
+    Axiom sendCCond: forall {c}, defined n -> defined c ->
                        parent c n ->
                        forall {m},
                          mark mch n c a t m ->
                          sle (to m) (state n a t) /\
-                         forall {c'}, c' <> c -> parent c' n -> sle (dir n c' a t)
+                         forall {c'}, defined c' -> 
+                                      c' <> c -> parent c' n -> sle (dir n c' a t)
                                       match to m with
                                         | Mo => In
                                         | Sh => Sh
                                         | In => Mo
                                       end.
-    Axiom oneRespC: forall {c1 c2},
+    Axiom oneRespC: forall {c1 c2}, defined n -> defined c1 -> defined c2 ->
                       parent c1 n -> parent c2 n ->
                       forall {m1}, (mark mch n c1 a t m1 \/ recv mch c1 n a t m1) ->
                                    forall {m2},
                                      (mark mch n c2 a t m2 \/ recv mch c2 n a t m2) -> c1 = c2.
-    Axiom respPNoRespC: forall {p}, parent n p ->
+    Axiom respPNoRespC: forall {p}, defined n -> defined p -> parent n p ->
                                     forall {m},
                                       (mark mch n p a t m \/ recv mch p n a t m) ->
-                                      forall {c}, parent c n -> forall mc,
+                                      forall {c}, defined c -> parent c n -> forall mc,
                                         ~ (mark mch n c a t mc \/ recv mch c n a t mc).
-    Axiom noParentSame: (forall {p}, ~ parent n p) -> state n a (S t) = state n a t.
+    Axiom noParentSame: defined n -> (forall {p}, defined p -> ~ parent n p) ->
+                        state n a (S t) = state n a t.
   End Node.
-  Axiom oneParent: forall {n p1 p2}, parent n p1 -> parent n p2 -> p1 = p2.
+  Axiom oneParent: forall {n p1 p2}, defined n -> defined p1 -> defined p2 ->
+                                     parent n p1 -> parent n p2 -> p1 = p2.
   Axiom initCompat:
-    forall {n c}, parent c n -> forall a, dir n c a 0 = In.
+    forall {n c}, defined n -> defined c -> parent c n -> forall a, dir n c a 0 = In.
 End CompatBehavior.
 
 Module Type CompatTheorem (dt: DataTypes) (ch: ChannelPerAddr dt).
   Import dt ch.
   Parameter compatible:
-    forall {n} a t {c}, parent c n ->
+    forall {n}, defined n -> forall a t {c}, defined c -> parent c n ->
                         sle (dir n c a t) (state n a t) /\
-                        forall {c'}, c' <> c -> parent c' n -> sle (dir n c' a t)
+                        forall {c'}, defined c' -> c' <> c -> parent c' n -> sle (dir n c' a t)
                                                                    match dir n c a t with
+                                                                     | Mo => In
+                                                                     | Sh => Sh
+                                                                     | In => Mo
+                                                                   end.
+  Parameter compat:
+    forall {n}, defined n -> forall a t {c}, defined c -> parent c n ->
+                        sle (state c a t) (state n a t) /\
+                        forall {c'}, defined c' -> c' <> c -> parent c' n -> sle (state c' a t)
+                                                                   match state c a t with
                                                                      | Mo => In
                                                                      | Sh => Sh
                                                                      | In => Mo
@@ -59,183 +70,209 @@ Module mkCompat (dt: DataTypes) (ch: ChannelPerAddr dt) (cb: CompatBehavior dt c
   Import dt ch cb ba mbt.
 
   Theorem compatible:
-    forall {n} a t {c}, parent c n ->
+    forall {n}, defined n -> forall a t {c}, defined c -> parent c n ->
                         sle (dir n c a t) (state n a t) /\
-                        forall {c'}, c' <> c -> parent c' n -> sle (dir n c' a t)
+                        forall {c'}, defined c' -> c' <> c -> parent c' n -> sle (dir n c' a t)
                                                                    match dir n c a t with
                                                                      | Mo => In
                                                                      | Sh => Sh
                                                                      | In => Mo
                                                                    end.
   Proof.
-    intros n a t.
+    intros n nDef a t.
     induction t.
-    intros c cond.
+    intros c cDef cond.
     constructor.
-    pose proof @initCompat n c cond a as c2.
+    pose proof @initCompat n c nDef cDef cond a as c2.
     rewrite c2.
     unfold sle; destruct (state n a 0); auto.
-    intros c' c'_ne_c c'Child.
-    pose proof @initCompat n c' c'Child a as c2.
+    intros c' c'Def c'_ne_c c'Child.
+    pose proof @initCompat n c' nDef c'Def c'Child a as c2.
     rewrite c2; destruct (dir n c a 0); unfold sle; auto.
-    destruct (classical (exists p m,
+    destruct (classical (exists p m, defined p /\
                            parent n p /\
                            (mark mch n p a t m \/ recv mch p n a t m))) as [respP|noRespP].
-    destruct respP as [p [m [p_parent markOrRecv]]].
-    pose proof @respPNoRespC n a t p p_parent m markOrRecv as noChild.
-    assert (sameDir: forall c, parent c n -> dir n c a t = dir n c a (S t)).
-    intros c c_child.
-    pose proof respPNoRespC p_parent markOrRecv c_child as noRespC.
+    destruct respP as [p [m [pDef [p_parent markOrRecv]]]].
+    pose proof @respPNoRespC n a t p nDef pDef p_parent m markOrRecv as noChild.
+    assert (sameDir: forall c, defined c -> parent c n -> dir n c a t = dir n c a (S t)).
+    intros c cDef c_child.
+    pose proof respPNoRespC nDef pDef p_parent markOrRecv cDef c_child as noRespC.
     assert (st_eq: dir n c a t = dir n c a (S t)).
     assert (stuff: {dir n c a t = dir n c a (S t)} + {dir n c a t <> dir n c a (S t)})
       by decide equality.
     destruct stuff as [eq|neq].
     assumption.
     assert (neq': dir n c a (S t) <> dir n c a t) by auto.
-    pose proof (change (@dt n c c_child) neq') as resp.
+    pose proof (change (@dt n c nDef cDef c_child) neq') as resp.
     generalize noRespC resp; clear; firstorder.
     assumption.
-    intros c c_child.
-    pose proof (sameDir c c_child) as dir_eq.
+    intros c cDef c_child.
+    pose proof (sameDir c cDef c_child) as dir_eq.
     rewrite <- dir_eq in *.
-    assert (sameC': forall c', c' <> c -> parent c' n -> dir n c' a t = dir n c' a (S t))
+    assert (sameC': forall c', defined c' -> c' <> c -> parent c' n -> dir n c' a t = dir n c' a (S t))
            by (generalize sameDir; clear; firstorder).
     destruct markOrRecv as [markm | recvm].
-    pose proof (sendPCond p_parent markm c_child) as dir_le_to_m.
-    pose proof (sendmChange (@st p n p_parent) markm) as sth.
+    pose proof (sendPCond nDef pDef p_parent markm cDef c_child) as dir_le_to_m.
+    pose proof (sendmChange (@st p n pDef nDef p_parent) markm) as sth.
     constructor.
 
     rewrite <- sth in dir_le_to_m.
     assumption.
 
-    intros.
-    specialize (sameC' c' H H0).
+    intros c' c'Def. intros.
+    specialize (sameC' c' c'Def H H0).
     rewrite <- sameC'.
-    generalize IHt c c_child H H0; clear; firstorder.
+    generalize IHt c cDef c_child c'Def H H0; clear; firstorder.
     constructor.
-    pose proof (cRecvUpgrade p_parent recvm) as st_lt.
-    generalize (IHt c c_child) st_lt; clear; intros.
+    pose proof (cRecvUpgrade pDef nDef p_parent recvm) as st_lt.
+    generalize (IHt c cDef c_child) st_lt; clear; intros.
     destruct H as [stuff _].
     unfold sle in *; unfold sle in *; destruct (dir n c a t); destruct (state n a t);
     destruct (state n a (S t)); auto.
-    intros c' c'Ne c'_child.
-    specialize (sameDir c' c'_child).
+    intros c' c'Def c'Ne c'_child.
+    specialize (sameDir c' c'Def c'_child).
     rewrite <- sameDir.
-    generalize IHt c'_child c'Ne c_child; clear; firstorder.
-    assert (noRespP': forall p, parent n p -> ~ ((exists m, mark mch n p a t m)
+    generalize IHt c'_child c'Def c'Ne cDef c_child; clear; firstorder.
+    assert (noRespP': forall p, defined p -> parent n p -> ~ ((exists m, mark mch n p a t m)
                                                    \/ (exists m, recv mch p n a t m)))
       by (
           generalize noRespP; clear; firstorder).
     assert (st_eq: state n a (S t) = state n a t).
-    destruct (classical (exists p, parent n p)) as [[p p_parent] | nop].
-    specialize (noRespP' p p_parent).
+    destruct (classical (exists p, defined p /\ parent n p)) as [[p [pDef p_parent]] | nop].
+    specialize (noRespP' p pDef p_parent).
     assert (eqOrNot: {state n a (S t) = state n a t} + {state n a (S t) <> state n a t}) by
         decide equality.
     destruct eqOrNot as [eq|not].
     assumption.
-    pose proof (noRespP' (change (@st p n p_parent) not)) as done.
+    pose proof (noRespP' (change (@st p n pDef nDef p_parent) not)) as done.
     firstorder.
-    assert (noP: forall p, ~ parent n p) by firstorder.
-    apply (@noParentSame n a t noP).
+    assert (noP: forall p, defined p -> ~ parent n p) by firstorder.
+    apply (@noParentSame n a t nDef noP).
     rewrite st_eq in *.
 
-    destruct (classical (exists c m, parent c n /\ (mark mch n c a t m \/ recv mch c n a t m))) as [ex|notEx].
-    destruct ex as [c [m [c_child resp]]].
-    assert (noneElse: forall c', c' <> c -> parent c' n ->
+    destruct (classical (exists c m, defined c /\ parent c n /\ (mark mch n c a t m \/ recv mch c n a t m))) as [ex|notEx].
+    destruct ex as [c [m [cDef [c_child resp]]]].
+    assert (noneElse: forall c', defined c' -> c' <> c -> parent c' n ->
                        ~ ((exists m, mark mch n c' a t m) \/ exists m, recv mch c' n a t m)).
-    intros c' c'_ne_c c'_child.
+    intros c' c'Def c'_ne_c c'_child.
     destruct (classical (exists m', mark mch n c' a t m' \/ recv mch c' n a t m'))
       as [ex|notEx].
     destruct ex as [m' sth].
-    pose proof (oneRespC c_child c'_child resp sth) as sth2.
+    pose proof (oneRespC nDef cDef c'Def c_child c'_child resp sth) as sth2.
     assert (c' = c) by auto.
     firstorder.
     firstorder.
-    assert (stEq: forall c', c' <> c -> parent c' n -> dir n c' a (S t) = dir n c' a t).
-    intros c' c'_ne_c c'_child.
-    specialize (noneElse c' c'_ne_c c'_child).
+    assert (stEq: forall c', defined c' -> c' <> c -> parent c' n -> dir n c' a (S t) = dir n c' a t).
+    intros c' c'Def c'_ne_c c'_child.
+    specialize (noneElse c' c'Def c'_ne_c c'_child).
     assert (eqOrNot: {dir n c' a (S t) = dir n c' a t} 
                      + {dir n c' a (S t) <> dir n c' a t}) by decide equality.
     destruct eqOrNot as [eq|not].
     assumption.
-    specialize (noneElse (change (@dt n c' c'_child) not)).
+    specialize (noneElse (change (@dt n c' nDef c'Def c'_child) not)).
     firstorder.
-    intros c0 c0_child.
+    intros c0 c0Def c0_child.
     destruct (classical (c0 = c)) as [c0_eq_c|c0_ne_c].
     rewrite c0_eq_c in *.
     destruct resp as [markm | recvm].
-    pose proof (sendmChange (@dt n c c_child) markm) as toM.
+    pose proof (sendmChange (@dt n c nDef cDef c_child) markm) as toM.
     rewrite toM.
-    pose proof (sendCCond c_child markm) as [stuff rest].
+    pose proof (sendCCond nDef cDef c_child markm) as [stuff rest].
     constructor.
     intuition.
-    intros.
-    specialize (stEq c' H H0).
+    intros c' c'Def. intros.
+    specialize (stEq c' c'Def H H0).
     rewrite stEq.
-    specialize (rest c' H H0).
+    specialize (rest c' c'Def H H0).
     intuition.
-    pose proof (pRecvDowngrade c_child recvm) as sth_gt.
+    pose proof (pRecvDowngrade nDef cDef c_child recvm) as sth_gt.
     constructor.
-    destruct (IHt c c_child) as [good bad].
+    destruct (IHt c cDef c_child) as [good bad].
     unfold slt in *; unfold sle in *; destruct (dir n c a (S t)); destruct (dir n c a t);
     destruct (state n a t); auto.
     clear c0 c0_child c0_eq_c.
-    intros c' c'_ne_c c'_child.
-    specialize (stEq c' c'_ne_c c'_child).
+    intros c' c'Def c'_ne_c c'_child.
+    specialize (stEq c' c'Def c'_ne_c c'_child).
     rewrite stEq in *; clear stEq.
-    destruct (IHt c c_child) as [_ rest]; clear IHt.
-    specialize (rest c' c'_ne_c c'_child).
+    destruct (IHt c cDef c_child) as [_ rest]; clear IHt.
+    specialize (rest c' c'Def c'_ne_c c'_child).
     unfold slt in *; unfold sle in *; destruct (dir n c a (S t)); destruct (dir n c a t);
     destruct (dir n c' a t); auto.
 
-    pose proof (stEq c0 c0_ne_c c0_child) as stEq'.
+    pose proof (stEq c0 c0Def c0_ne_c c0_child) as stEq'.
     rewrite stEq'.
     constructor.
-    generalize IHt c0_child; clear; firstorder.
-    intros c' c'_ne_c0 c'_child.
+    generalize IHt c0Def c0_child; clear; firstorder.
+    intros c' c'Def c'_ne_c0 c'_child.
     destruct (classical (c' = c)) as [c'_eq_c | c'_ne_c].
     rewrite c'_eq_c in *.
     destruct resp as [markm | recvm].
-    pose proof (sendCCond c_child markm) as [_ toMOld].
+    pose proof (sendCCond nDef cDef c_child markm) as [_ toMOld].
     assert (c_ne_c0: c0 <> c) by auto.
-    specialize (toMOld c0 c_ne_c0 c0_child).
+    specialize (toMOld c0 c0Def c_ne_c0 c0_child).
     rewrite <- c'_eq_c in *; clear c'_eq_c.
-    pose proof (sendmChange (dt c'_child) markm) as sth.
+    pose proof (sendmChange (dt nDef c'Def c'_child) markm) as sth.
     rewrite sth.
     destruct (dir n c0 a t); destruct (to m); unfold sle in *; auto.
 
-    pose proof (pRecvDowngrade c_child recvm) as sth_gt.
+    pose proof (pRecvDowngrade nDef cDef c_child recvm) as sth_gt.
     assert (gtz: slt In (dir n c a t)) by
         (destruct (dir n c a (S t)); destruct (dir n c a t); unfold slt in *; auto).
-    pose proof (IHt c0 c0_child) as [_ sth1].
-    specialize (sth1 c c'_ne_c0 c_child).
+    pose proof (IHt c0 c0Def c0_child) as [_ sth1].
+    specialize (sth1 c c'Def c'_ne_c0 c_child).
     unfold slt in *; unfold sle in *; destruct (dir n c a (S t));
     destruct (dir n c0 a t); destruct (dir n c a t); auto.
 
-    specialize (stEq c' c'_ne_c c'_child).
+    specialize (stEq c' c'Def c'_ne_c c'_child).
     rewrite stEq.
-    generalize IHt c0_child c'_ne_c0 c'_child; clear; firstorder.
+    generalize IHt c0_child c'Def c0Def c'_ne_c0 c'_child; clear; firstorder.
 
-    assert (same: forall c, parent c n -> dir n c a (S t) = dir n c a t).
-    intros c c_child.
+    assert (same: forall c, defined c -> parent c n -> dir n c a (S t) = dir n c a t).
+    intros c cDef c_child.
     assert (eqOrNot: {dir n c a (S t) = dir n c a t} + {dir n c a (S t) <> dir n c a t})
            by decide equality.
     destruct eqOrNot as [eq|not].
     assumption.
-    pose proof (change (@dt n c c_child) not) as ppp.
-    generalize notEx c_child ppp; clear; firstorder.
+    pose proof (change (@dt n c nDef cDef c_child) not) as ppp.
+    generalize notEx nDef cDef c_child ppp; clear; firstorder.
 
-    intros c c_child.
+    intros c cDef c_child.
     constructor.
-    specialize (same c c_child).
+    specialize (same c cDef c_child).
     rewrite same.
-    generalize IHt c_child; clear; firstorder.
+    generalize IHt cDef c_child; clear; firstorder.
 
-    intros.
-    pose proof (same c' H0) as dunk.
+    intros c' c'Def. intros.
+    pose proof (same c' c'Def H0) as dunk.
     rewrite dunk.
-    pose proof (same c c_child) as dukn.
+    pose proof (same c cDef c_child) as dukn.
     rewrite dukn in *.
-    generalize IHt c_child H H0; clear; firstorder.
+    generalize IHt cDef c'Def c_child H H0; clear; firstorder.
   Qed.
+
+  Theorem compat:
+    forall {n}, defined n -> forall a t {c}, defined c -> parent c n ->
+                        sle (state c a t) (state n a t) /\
+                        forall {c'}, defined c' -> c' <> c -> parent c' n -> sle (state c' a t)
+                                                                   match state c a t with
+                                                                     | Mo => In
+                                                                     | Sh => Sh
+                                                                     | In => Mo
+                                                                   end.
+  Proof.
+    intros n nDef a t c cDef c_child.
+    pose proof (compatible nDef a t cDef c_child) as base.
+    constructor.
+    destruct base as [dr _].
+    pose proof (conservative nDef cDef c_child a t) as dLe.
+    apply (sle_sle_sle dLe dr).
+    destruct base as [_ others].
+    intros c' c'Def c'_ne p_c'.
+    specialize (others c' c'Def c'_ne p_c').
+    pose proof (conservative nDef cDef c_child a t) as st.
+    pose proof (conservative nDef c'Def p_c' a t) as st'.
+    unfold sle in *; destruct (state c' a t); destruct (state c a t);
+    destruct (dir n c' a t); destruct (dir n c a t); auto.
+  Qed.
+
 End mkCompat.
