TwoLevel.v
@@ -3,35 +3,37 @@ Require Import DataTypes Useful Channel Cache Compatible L1.
 Module Type LatestValueAxioms (dt: DataTypes) (ch: ChannelPerAddr dt) (l1: L1Axioms dt).
   Import dt ch l1.
 
-  Axiom toChild: forall {n a t p m},
+  Axiom toChild: forall {n a t p m}, defined n -> defined p ->
                    parent n p -> 
                    mark mch p n a t m -> from m = In -> dataM m = data p a t.
-  Axiom fromParent: forall {n a t p m},
+  Axiom fromParent: forall {n a t p m}, defined n -> defined p ->
                       parent n p -> 
                       recv mch p n a t m -> from m = In -> data n a (S t) = dataM m.
-  Axiom toParent: forall {n a t c m},
+  Axiom toParent: forall {n a t c m}, defined n -> defined c ->
                      parent c n ->
                      mark mch c n a t m -> slt Sh (from m) -> dataM m = data c a t.
-  Axiom fromChild: forall {n a t c m},
+  Axiom fromChild: forall {n a t c m}, defined n -> defined c ->
                      parent c n ->
                      recv mch c n a t m -> slt Sh (from m) -> data n a (S t) = dataM m.
-  Axiom initLatest: forall {n} a, (forall {p}, ~ parent n p) -> data n a 0 = Initial
-                                                                /\ state n a 0 = Mo.
+  Axiom initLatest: forall {n} a, defined n -> (forall {p}, defined p -> ~ parent n p)
+                                  -> data n a 0 = Initial /\ state n a 0 = Mo.
 
-  Axiom deqImpData: forall {n a t l i}, deqR n l a St i t -> data n a (S t) = Store l.
+  Axiom deqImpData: forall {n a t l i}, defined n -> deqR n l a St i t ->
+                                        data n a (S t) = Store l.
 
   Axiom changeData:
-    forall {n a t},
+    forall {n a t}, defined n ->
       data n a (S t) <> data n a t ->
-      (exists m, (exists p, parent n p /\ recv mch p n a t m /\ from m = In) \/
-                 (exists c, parent c n /\ recv mch c n a t m /\ slt Sh (from m))) \/
+      (exists m, (exists p, defined p /\ parent n p /\ recv mch p n a t m /\ from m = In) \/
+                 (exists c, defined c /\ parent c n /\ recv mch c n a t m /\
+                            slt Sh (from m))) \/
       exists l i, deqR n l a St i t.
 
 
-  Axiom deqImpNoSend: forall {c l a d i t}, deqR c l a d i t ->
-                                            forall {m p}, ~ mark mch c p a t m.
-  Axiom deqImpNoRecv: forall {c l a d i t}, deqR c l a d i t ->
-                                            forall {m p}, ~ recv mch p c a t m. 
+  Axiom deqImpNoSend: forall {c l a d i t}, defined c -> deqR c l a d i t ->
+                                            forall {m p}, defined p -> ~ mark mch c p a t m.
+  Axiom deqImpNoRecv: forall {c l a d i t}, defined c -> deqR c l a d i t ->
+                                            forall {m p}, defined p -> ~ recv mch p c a t m. 
 End LatestValueAxioms.
 
 Module LatestValueTheorems (dt: DataTypes) (ch: ChannelPerAddr dt) (c: BehaviorAxioms dt ch)
@@ -41,73 +43,77 @@ Module LatestValueTheorems (dt: DataTypes) (ch: ChannelPerAddr dt) (c: BehaviorA
   Import dt ch c l1 comp lv mbt cbt.
 
   Theorem uniqM:
-    forall {c a t},
+    forall {c a t}, defined c ->
       leaf c ->
-      state c a t = Mo -> forall {co}, leaf co -> c <> co -> state co a t = In.
+      state c a t = Mo -> forall {co}, defined co -> leaf co -> c <> co -> state co a t = In.
   Proof.
-    intros c a t leaf_c c_M co leaf_co c_ne_co.
+    intros c a t cDef leaf_c c_M co coDef leaf_co c_ne_co.
     pose proof (who'Parent c leaf_c) as c_parent.
     pose proof (who'Parent co leaf_co) as co_parent.
-    pose proof (conservative c_parent a t) as cLe.
-    pose proof (conservative co_parent a t) as coLe.
-    pose proof (@compatible Parent a t c c_parent) as [_ comp].
+    pose proof (conservative defParent cDef c_parent a t) as cLe.
+    pose proof (conservative defParent coDef co_parent a t) as coLe.
+    pose proof (@compatible Parent defParent a t c cDef c_parent) as [_ comp].
     assert (dirM: dir Parent c a t = Mo) by
         ( unfold sle in *; destruct (state c a t); destruct (dir Parent c a t); firstorder;
           discriminate).
     assert (co_ne_c: co <> c) by auto.
-    specialize (comp co co_ne_c co_parent).
+    specialize (comp co coDef co_ne_c co_parent).
     rewrite dirM in comp.
     unfold sle in *; destruct (dir Parent co a t); destruct (state co a t); firstorder.
   Qed.
 
   Section ForAddr.
     Context {a: Addr}.
-    Theorem allLatestValue: forall {t n},
-      (sle Sh (state n a t) /\ forall {c}, parent c n -> sle (dir n c a t) Sh) ->
+    Theorem allLatestValue: forall {t n}, defined n ->
+      (sle Sh (state n a t) /\ forall {c}, defined c -> parent c n -> sle (dir n c a t) Sh) ->
       match data n a t with
-        | Initial => forall {ti}, 0 <= ti < t -> forall {ci li ii}, ~ deqR ci li a St ii ti
+        | Initial => forall {ti}, 0 <= ti < t -> forall {ci li ii}, defined ci ->
+                                                                    ~ deqR ci li a St ii ti
         | Store lb =>
-          exists cb ib tb, tb < t /\ deqR cb lb a St ib tb /\
+          exists cb ib tb, defined cb /\ tb < t /\ deqR cb lb a St ib tb /\
                            forall {ti}, tb < ti < t ->
-                                        forall {ci li ii}, ~ deqR ci li a St ii ti
+                                        forall {ci li ii}, defined ci ->
+                                                           ~ deqR ci li a St ii ti
       end.
     Proof.
-      pose (fun t => forall n,
+      pose (fun t => forall n, defined n ->
               sle Sh (state n a t) /\
-              (forall c, parent c n -> sle (dir n c a t) Sh) ->
+              (forall c, defined c -> parent c n -> sle (dir n c a t) Sh) ->
                          match data n a t with
                            | Initial =>
                              forall ti : nat,
                                0 <= ti < t ->
                                forall (ci : Cache) (li : Label) (ii : Index),
-                                 ~ deqR ci li a St ii ti
+                                 defined ci -> ~ deqR ci li a St ii ti
                            | Store lb =>
                              exists (cb : Cache) (ib : Index) (tb : nat),
-                               tb < t /\
+                               defined cb /\ tb < t /\
                                deqR cb lb a St ib tb /\
                                (forall ti : nat,
                                   tb < ti < t ->
                                   forall (ci : Cache) (li : Label) (ii : Index),
-                                    ~ deqR ci li a St ii ti)
+                                    defined ci -> ~ deqR ci li a St ii ti)
                          end) as P.
-      pose proof (initLatest a noParentHasParent) as [pInit pM].
+      pose proof (initLatest a defParent noParentHasParent) as [pInit pM].
       apply (@ind P).
       unfold P in *; clear P.
-      assert (childIn: forall n, state (Child n) a 0 = In).
-      intros c.
+      assert (childIn: forall n, defined (Child n) -> state (Child n) a 0 = In).
+      intros c cDef.
       assert (pChilds: parent (Child c) Parent) by
           (unfold parent; auto).
-      pose proof (initCompat pChilds a) as dirIn.
-      pose proof (conservative pChilds a 0) as sleSt.
+      pose proof (initCompat defParent cDef pChilds a) as dirIn.
+      pose proof (conservative defParent cDef pChilds a 0) as sleSt.
       unfold sle in *; destruct (dir Parent (Child c) a 0); destruct (state (Child c) a 0);
       firstorder; discriminate.
-      intros n.
+      intros n nDef.
       induction n.
       rewrite pInit.
       unfold not; intros.
       assert (ti0: ti = 0) by omega.
       rewrite ti0 in *.
-      pose proof (deqLeaf H1) as leafC.
+      omega.
+(*
+      pose proof (deqLeaf nDef H1) as leafC.
       unfold leaf in leafC.
       destruct ci.
       assumption.
@@ -115,44 +121,47 @@ Module LatestValueTheorems (dt: DataTypes) (ch: ChannelPerAddr dt) (c: BehaviorA
       pose proof (processDeq H1) as contra.
       rewrite childIn in contra.
       discriminate.
-      specialize (childIn n).
+*)
+      specialize (childIn n nDef).
       intros H.
       rewrite childIn in H.
       unfold sle in *; firstorder.
       unfold P in *; clear P.
-      intros t SIHt n H.
+      intros t SIHt n nDef H.
       assert (stEq: forall t, state Parent a t = Mo) by
-          (intros t'; pose proof (noParentNoStChange a t' noParentHasParent); rewrite <- pM in *;
+          (intros t'; pose proof (noParentNoStChange a t' defParent noParentHasParent); rewrite <- pM in *;
           auto).
       destruct n.
-      destruct (classical (forall c, parent c Parent -> sle (dir Parent c a t) Sh)) as
+      destruct (classical (forall c, defined c -> parent c Parent -> sle (dir Parent c a t) Sh)) as
           [prevLatest|prevNotLatest].
       assert (stM: sle Sh (state Parent a t)) by (specialize (stEq t);
                                                    rewrite stEq; unfold sle; auto).
       assert (cond: t <= t) by omega.
-      specialize (SIHt t cond Parent (conj stM prevLatest)); clear cond stM.
+      specialize (SIHt t cond Parent defParent (conj stM prevLatest)); clear cond stM.
       destruct H as [_ dirSmall].
-      assert (cSmall: forall c, parent c Parent -> sle (state c a t) Sh).
-      intros c c_child.
-      specialize (prevLatest c c_child).
-      pose proof (conservative c_child a t) as help.
+      assert (cSmall: forall c, defined c -> parent c Parent -> sle (state c a t) Sh).
+      intros c cDef c_child.
+      specialize (prevLatest c cDef c_child).
+      pose proof (conservative defParent cDef c_child a t) as help.
       unfold sle in *; destruct (state c a t); destruct (dir Parent c a t); auto.
-      assert (noDeq: forall ci li ii, ~ deqR ci li a St ii t) by
-          (unfold not; intros ci li ii H;
+      assert (noDeq: forall ci li ii, defined ci -> ~ deqR ci li a St ii t) by
+          (unfold not; intros ci li ii ciDef H;
            pose proof (processDeq H) as sth; simpl in *;
                                              pose proof (deqLeaf H) as leaf_ci;
            assert (ci_child: parent ci Parent) by (unfold parent; unfold leaf in *;
                                                                   destruct ci; auto);
-           specialize (cSmall ci ci_child); rewrite sth in cSmall; unfold sle; auto).
+           specialize (cSmall ci ciDef ci_child); rewrite sth in cSmall; unfold sle; auto).
       destruct (classical (data Parent a (S t) = data Parent a t)) as [e1|e2].
       rewrite e1.
       destruct (data Parent a t).
       intros ti cond.
       assert (H: 0 <= ti < t \/ ti = t) by omega.
       destruct H as [one|two]; [firstorder| rewrite two in *; firstorder].
-      destruct SIHt as [cb [ib [tb [tb_lt_t [deqTb rest]]]]].
+      destruct SIHt as [cb [ib [tb [cbDef [tb_lt_t [deqTb rest]]]]]].
       exists cb; exists ib; exists tb.
       assert (sth: tb < S t) by omega.
+      constructor.
+      assumption.
       constructor.
       assumption.
       constructor.
@@ -162,47 +171,48 @@ Module LatestValueTheorems (dt: DataTypes) (ch: ChannelPerAddr dt) (c: BehaviorA
       destruct H as [one|two].
       apply (rest ti one).
       rewrite two in *; assumption.
-      pose proof (changeData e2) as sth.
+      pose proof (changeData nDef e2) as sth.
       destruct sth as [sth|deqSth].
-      destruct sth as [m [[p [parentp _]]|recvFromC]].
-      pose proof (noParentHasParent p parentp).
+      destruct sth as [m [[p [defP [parentp _]]]|recvFromC]].
+      pose proof (noParentHasParent p defP parentp).
       firstorder.
-      destruct recvFromC as [c [c_child [recvm sltFromM]]].
-      pose proof (recvmCond c_child recvm) as contra.
-      specialize (prevLatest c c_child).
+      destruct recvFromC as [c [cDef [c_child [recvm sltFromM]]]].
+      pose proof (recvmCond defParent cDef c_child recvm) as contra.
+      specialize (prevLatest c cDef c_child).
       rewrite <- contra in prevLatest.
       unfold sle in *; unfold slt in *; destruct (from m); firstorder; discriminate.
       destruct deqSth as [l [i deqSth]].
       pose proof (deqLeaf deqSth) as H.
       unfold leaf in H; firstorder.
-      destruct (classical (exists c, parent c Parent /\ ~ sle (dir Parent c a t) Sh))
-               as [[c [c_child dirHigh]]|notEx].
+      destruct (classical (exists c, defined c /\ parent c Parent /\
+                                     ~ sle (dir Parent c a t) Sh))
+               as [[c [cDef [c_child dirHigh]]]|notEx].
       destruct H as [_ cacheLow].
-      specialize (cacheLow c c_child).
+      specialize (cacheLow c cDef c_child).
       assert (downgrade: slt (dir Parent c a (S t)) (dir Parent c a t)) by
           (unfold slt in *; unfold sle in *; destruct (dir Parent c a (S t));
            destruct (dir Parent c a t); auto).
       pose proof (slt_neq' downgrade) as neq.
-      pose proof (change (dt c_child) neq) as [[m markm] | [m recvm]].
-      pose proof (pSendUpgrade c_child markm) as upg.
+      pose proof (change (dt defParent cDef c_child) neq) as [[m markm] | [m recvm]].
+      pose proof (pSendUpgrade defParent cDef c_child markm) as upg.
       pose proof (slt_slti_false downgrade upg) as f.
       firstorder.
       pose proof (recvImpMark recvm) as [ts [ts_le_t sendm]].
 
 
-      pose proof (sendmFrom (st c_child) sendm) as fromX.
-      pose proof (sendmChange (st c_child) sendm) as toM.
-      pose proof (cSendDowngrade c_child sendm) as dgd.
+      pose proof (sendmFrom (st defParent cDef c_child) sendm) as fromX.
+      pose proof (sendmChange (st defParent cDef c_child) sendm) as toM.
+      pose proof (cSendDowngrade defParent cDef c_child sendm) as dgd.
       assert (pHigh: forall tx, ts < tx < S t -> slt In (dir Parent c a tx)).
       intros tx cond; assert (cond2: ts <= tx <= t) by omega;
-      pose proof (cSendPGreaterState c_child sendm recvm cond2) as sth.
+      pose proof (cSendPGreaterState defParent cDef c_child sendm recvm cond2) as sth.
       rewrite fromX in sth.
       unfold slt in *; unfold sle in *; destruct (state c a (S ts));
       destruct (state c a ts); destruct (dir Parent c a tx); auto.
 
       assert (cLow: forall tx, ts < tx < S t -> slt (state c a tx) Mo).
       intros tx cond; assert (cond2: ts < tx <= t) by omega;
-      pose proof (cSendCSmallerState c_child sendm recvm cond2) as sth.
+      pose proof (cSendCSmallerState defParent cDef c_child sendm recvm cond2) as sth.
       rewrite <- toM in sth.
       unfold slt in *; unfold sle in *; destruct (state c a (S ts));
       destruct (state c a tx); auto.
@@ -210,65 +220,66 @@ Module LatestValueTheorems (dt: DataTypes) (ch: ChannelPerAddr dt) (c: BehaviorA
 
 
       assert (others: forall tx, ts < tx < S t ->
-                                 forall c', c' <> c -> parent c' Parent ->
+                                 forall c', defined c' -> c' <> c -> parent c' Parent ->
                                             sle (dir Parent c' a tx)
                                                 match dir Parent c a tx with
                                                   | In => Mo
                                                   | Sh => Sh
                                                   | Mo => In
                                                 end) by
-          (intros tx _; apply (compatible a tx c_child)).
+          (intros tx _; apply (compatible defParent a tx cDef c_child)).
       assert (c'DirLow:
                 forall tx,
                   ts < tx < S t -> 
-                  forall c', c' <> c -> parent c' Parent -> slt (dir Parent c' a tx) Mo).
-      intros tx cond c' c'_ne_c c'_child.
-      specialize (others tx cond c' c'_ne_c c'_child).
+                  forall c', defined c' -> c' <> c ->
+                             parent c' Parent -> slt (dir Parent c' a tx) Mo).
+      intros tx cond c' c'Def c'_ne_c c'_child.
+      specialize (others tx cond c' c'Def c'_ne_c c'_child).
       specialize (pHigh tx cond).
       unfold slt in *; destruct (dir Parent c a tx); destruct (dir Parent c' a tx); auto.
-      assert (c'Low: forall tx, ts < tx < S t -> forall c',
+      assert (c'Low: forall tx, ts < tx < S t -> forall c', defined c' ->
                                                    c' <> c ->
                                                    parent c' Parent ->
                                                    slt (state c' a tx) Mo).
-      intros tx cond c' c'_ne_c c'_child.
-      specialize (c'DirLow tx cond c' c'_ne_c c'_child).
-      pose proof (conservative c'_child a tx) as sig.
+      intros tx cond c' c'Def c'_ne_c c'_child.
+      specialize (c'DirLow tx cond c' c'Def c'_ne_c c'_child).
+      pose proof (conservative defParent c'Def c'_child a tx) as sig.
       unfold slt in *; destruct (dir Parent c' a tx); destruct (state c' a tx); auto.
-      assert (allLow: forall tx, ts < tx < S t -> forall c0,
+      assert (allLow: forall tx, ts < tx < S t -> forall c0, defined c0 ->
                                            parent c0 Parent -> slt (state c0 a tx) Mo).
-      intros tx cond c0 c0_child.
+      intros tx cond c0 c0Def c0_child.
       assert (cache: {c0 = c} + {c0 <> c}) by (
                                         decide equality;
                                         decide equality).
       destruct cache as [eq|notEq].
       rewrite eq in *; apply (cLow tx cond).
-      apply (c'Low tx cond c0 notEq c0_child).
+      apply (c'Low tx cond c0 c0Def notEq c0_child).
       assert (noSt: forall ti, ts < ti < S t ->
-                               forall ci li ii, ~ deqR ci li a St ii ti).
-      unfold not; intros ti cond ci li ii deqSt.
+                               forall ci li ii, defined ci -> ~ deqR ci li a St ii ti).
+      unfold not; intros ti cond ci li ii ciDef deqSt.
       pose proof (deqLeaf deqSt) as leafCi.
       assert(ci_child: parent ci Parent) by (unfold leaf in *; unfold parent in *; auto).
       pose proof (processDeq deqSt) as mustMo.
       simpl in *.
-      specialize (allLow ti cond ci ci_child).
+      specialize (allLow ti cond ci ciDef ci_child).
       unfold sle in allLow; destruct (state ci a ti); auto; discriminate.
       pose proof (not_sle_slt dirHigh) as dirHigh'.
-      pose proof (recvmCond c_child recvm) as fromM.
+      pose proof (recvmCond defParent cDef c_child recvm) as fromM.
       rewrite <- fromM in dirHigh'.
-      pose proof (toParent c_child sendm dirHigh') as dM.
-      pose proof (fromChild c_child recvm dirHigh') as dM'.
+      pose proof (toParent defParent cDef c_child sendm dirHigh') as dM.
+      pose proof (fromChild defParent cDef c_child recvm dirHigh') as dM'.
       rewrite <- dM' in dM; rewrite dM.
       assert (le: ts <= t) by omega.
-      pose proof (sendmFrom (st c_child) sendm) as fromM'.
+      pose proof (sendmFrom (st defParent cDef c_child) sendm) as fromM'.
       rewrite fromM' in dirHigh'.
       assert (stCond: sle Sh (state c a ts)) by
           (
             destruct (state c a ts); unfold sle in *; unfold slt in *; auto;
             discriminate).
-      assert (cond2: forall c0, parent c0 c -> sle (dir c c0 a ts) Sh) by
-          (intros c0 c0_child; unfold parent in *; destruct c; destruct c0;
+      assert (cond2: forall c0, defined c0 -> parent c0 c -> sle (dir c c0 a ts) Sh) by
+          (intros c0 c0Def c0_child; unfold parent in *; destruct c; destruct c0;
            assert (f: False) by auto; firstorder).
-      pose proof (SIHt ts le c (conj stCond cond2)) as useful.
+      pose proof (SIHt ts le c cDef (conj stCond cond2)) as useful.
       destruct (data c a ts).
       intros ti cond1.
 
@@ -279,26 +290,26 @@ Module LatestValueTheorems (dt: DataTypes) (ch: ChannelPerAddr dt) (c: BehaviorA
       destruct cond3 as [e1|[e2|e3]].
       generalize noSt e1 useful; clear; firstorder.
       generalize noSt e2 useful; clear; firstorder.
-      unfold not; rewrite e3 in *; intros ci li ii deqSt.
+      unfold not; rewrite e3 in *; intros ci li ii ciDef deqSt.
       assert (eqOrNot: c = ci \/ c <> ci) by (decide equality ; decide equality ).
       destruct eqOrNot as [eq|notEq].
       rewrite eq in *.
-      apply (deqImpNoSend deqSt sendm).
+      apply (deqImpNoSend ciDef deqSt defParent sendm).
       pose proof (processDeq deqSt) as stte.
       simpl in stte.
       pose proof (deqLeaf deqSt) as leafCi.
       assert (c'_child: parent ci Parent) by (unfold parent; unfold leaf in *; destruct ci;
                                               auto).
-      pose proof (conservative c'_child a ts) as cons.
+      pose proof (conservative defParent ciDef c'_child a ts) as cons.
       rewrite stte in cons.
       assert (dirM: dir Parent ci a ts = Mo) by (unfold sle in cons;
                                                  destruct (dir Parent ci a ts); firstorder).
-      pose proof (compatible a ts c'_child) as [_ otherCaches].
+      pose proof (compatible defParent a ts ciDef c'_child) as [_ otherCaches].
       rewrite dirM in otherCaches.
-      specialize (otherCaches c notEq c_child).
+      specialize (otherCaches c cDef notEq c_child).
       assert (dirIn: dir Parent c a ts = In) by (unfold sle in *; destruct (dir Parent c a ts);
                                                  firstorder).
-      pose proof (conservative c_child a ts) as cons2.
+      pose proof (conservative defParent cDef c_child a ts) as cons2.
       rewrite dirIn in cons2.
       assert (cIn: state c a ts = In) by (unfold sle in cons2; destruct (state c a ts) ;
                                                                firstorder).
@@ -308,9 +319,10 @@ Module LatestValueTheorems (dt: DataTypes) (ch: ChannelPerAddr dt) (c: BehaviorA
 
 
 
-      destruct useful as [cb [ib [tb [tbTs [deqTb rest]]]]].
+      destruct useful as [cb [ib [tb [cbDef [tbTs [deqTb rest]]]]]].
       exists cb; exists ib; exists tb.
       assert (tsLeSt: ts <= S t) by omega.
+      constructor. assumption.
       constructor. 
       assert (tb < S t) by omega.
       assumption.
@@ -321,26 +333,26 @@ Module LatestValueTheorems (dt: DataTypes) (ch: ChannelPerAddr dt) (c: BehaviorA
       generalize rest e1 noSt; clear; firstorder.
       generalize rest e2 noSt; clear; firstorder.
 
-      unfold not; rewrite e3 in *; intros ci li ii deqSt.
+      unfold not; rewrite e3 in *; intros ci li ii ciDef deqSt.
       assert (eqOrNot: c = ci \/ c <> ci) by (decide equality ; decide equality ).
       destruct eqOrNot as [eq|notEq].
       rewrite eq in *.
-      apply (deqImpNoSend deqSt sendm).
+      apply (deqImpNoSend ciDef deqSt defParent sendm).
       pose proof (processDeq deqSt) as stte.
       simpl in stte.
       pose proof (deqLeaf deqSt) as leafCi.
       assert (c'_child: parent ci Parent) by (unfold parent; unfold leaf in *; destruct ci;
                                               auto).
-      pose proof (conservative c'_child a ts) as cons.
+      pose proof (conservative defParent ciDef c'_child a ts) as cons.
       rewrite stte in cons.
       assert (dirM: dir Parent ci a ts = Mo) by (unfold sle in cons;
                                                  destruct (dir Parent ci a ts); firstorder).
-      pose proof (compatible a ts c'_child) as [_ otherCaches].
+      pose proof (compatible defParent a ts ciDef c'_child) as [_ otherCaches].
       rewrite dirM in otherCaches.
-      specialize (otherCaches c notEq c_child).
+      specialize (otherCaches c cDef notEq c_child).
       assert (dirIn: dir Parent c a ts = In) by (unfold sle in *; destruct (dir Parent c a ts);
                                                  firstorder).
-      pose proof (conservative c_child a ts) as cons2.
+      pose proof (conservative defParent cDef c_child a ts) as cons2.
       rewrite dirIn in cons2.
       assert (cIn: state c a ts = In) by (unfold sle in cons2; destruct (state c a ts) ;
                                                                firstorder).
@@ -349,52 +361,57 @@ Module LatestValueTheorems (dt: DataTypes) (ch: ChannelPerAddr dt) (c: BehaviorA
 
 
 
-      assert (contra: forall c, parent c Parent -> ~ ~ sle (dir Parent c a t) Sh) by
+      assert (contra: forall c, defined c -> parent c Parent ->
+                                ~ ~ sle (dir Parent c a t) Sh) by
           firstorder.
-      assert (contra2: forall c, parent c Parent -> sle (dir Parent c a t) Sh) by
-          (intros c parentC;
-           specialize (contra c parentC);
+      assert (contra2: forall c, defined c -> parent c Parent -> sle (dir Parent c a t) Sh) by
+          (intros c cDef parentC;
+           specialize (contra c cDef parentC);
            unfold sle in *; destruct (dir Parent c a t); auto).
       firstorder.
 
       destruct H as [H _].
-      assert (noChildren: forall c, parent c (Child n) -> False) by
+      assert (noChildren: forall c, defined c -> parent c (Child n) -> False) by
          ( intros c c_parent; unfold parent in *; destruct c; auto ).
       destruct (classical (sle Sh (state (Child n) a t))) as [easy|hard].
       assert (ob: t <= t) by omega.
-      assert (contra: forall c, parent c (Child n) -> sle (dir (Child n) c a t) Sh) by
+      assert (contra: forall c, defined c -> 
+                                parent c (Child n) -> sle (dir (Child n) c a t) Sh) by
           (generalize noChildren; clear; firstorder).
-      specialize (SIHt t ob (Child n) (conj easy contra)).
+      specialize (SIHt t ob (Child n) nDef (conj easy contra)).
       assert (c_child: parent (Child n) Parent) by (unfold parent; auto).
-      pose proof (conservative c_child a t) as cons.
-      pose proof (compatible a t c_child) as [_ dirLow].
-      assert (others: forall c', c' <> Child n -> leaf c' -> sle (state c' a t) Sh).
-      intros c' c'_ne leaf_c'.
+      pose proof (conservative defParent nDef c_child a t) as cons.
+      pose proof (compatible defParent a t nDef c_child) as [_ dirLow].
+      assert (others: forall c', defined c' -> 
+                                 c' <> Child n -> leaf c' -> sle (state c' a t) Sh).
+      intros c' c'Def c'_ne leaf_c'.
       assert (c'_child: parent c' Parent) by (unfold parent in *; unfold leaf in *; auto).
-      specialize (dirLow c' c'_ne c'_child).
-      pose proof (conservative c'_child a t) as cons2.
+      specialize (dirLow c' c'Def c'_ne c'_child).
+      pose proof (conservative defParent c'Def c'_child a t) as cons2.
       unfold sle in *; destruct (state c' a t); destruct (dir Parent c' a t);
       destruct (state (Child n) a t); destruct (dir Parent (Child n) a t); auto.
-      assert (otherDeq: forall c', c' <> Child n -> forall li ii, ~ deqR c' li a St ii t).
-      unfold not; intros c' c'_ne li ii deqSt.
+      assert (otherDeq: forall c', defined c' ->
+                                   c' <> Child n -> forall li ii, ~ deqR c' li a St ii t).
+      unfold not; intros c' c'Def c'_ne li ii deqSt.
       pose proof (deqLeaf deqSt) as c'_leaf.
-      specialize (others c' c'_ne c'_leaf).
+      specialize (others c' c'Def c'_ne c'_leaf).
       pose proof (processDeq deqSt) as M; simpl in *.
       rewrite M in others; unfold sle in others; auto.
       destruct (classical (exists li ii, deqR (Child n) li a St ii t)) as
           [[li [ii deqSt]]|notEx].
-      pose proof (deqImpData deqSt) as newData.
+      pose proof (deqImpData nDef deqSt) as newData.
       rewrite newData in *.
       exists (Child n); exists ii; exists t.
       assert (t_lt_St: t < S t) by omega.
+      constructor. assumption.
       constructor. assumption.
       constructor. assumption.
       intros ti [c1 c2].
       assert (f: False) by omega.
       firstorder.
       assert (forall li ii, ~ deqR (Child n) li a St ii t) by firstorder.
-      assert (noDeq: forall c0 li ii, ~ deqR c0 li a St ii t).
-      intros c0 li ii.
+      assert (noDeq: forall c0 li ii, defined c0 -> ~ deqR c0 li a St ii t).
+      intros c0 li ii c0Def.
       assert ({c0 = Child n} + {c0 <> Child n}) by (decide equality; decide equality).
       destruct H1 as [eq|neq].
       rewrite eq in *.
@@ -408,8 +425,9 @@ Module LatestValueTheorems (dt: DataTypes) (ch: ChannelPerAddr dt) (c: BehaviorA
       destruct mur1 as [easy2|hard].
       apply (SIHt ti easy2).
       rewrite hard in *; firstorder.
-      destruct SIHt as [cb [ib [tb [tbLt [deqSt rest]]]]].
+      destruct SIHt as [cb [ib [tb [cbDef [tbLt [deqSt rest]]]]]].
       exists cb; exists ib; exists tb.
+      constructor. assumption.
       constructor. assert (tb < S t) by omega. assumption.
       constructor. assumption.
       intros ti cond.
@@ -417,24 +435,25 @@ Module LatestValueTheorems (dt: DataTypes) (ch: ChannelPerAddr dt) (c: BehaviorA
       destruct mur1 as [easy2|hard].
       apply (rest ti easy2).
       rewrite hard in *; firstorder.
-      pose proof (changeData neq) as [[m [fromParent|toChild]]| deqSt].
-      destruct fromParent as [p [p_parent [recvm fromM]]].
+      pose proof (changeData nDef neq) as [[m [fromParent|toChild]]| deqSt].
+      destruct fromParent as [p [pDef [p_parent [recvm fromM]]]].
       pose proof (recvImpMark recvm) as [ts [ts_le_t sendm]].
-      pose proof (sendmFrom (dt p_parent) sendm) as fromM'.
-      pose proof (cRecvRespPrevState p_parent recvm sendm) as same.
+      pose proof (sendmFrom (dt pDef nDef p_parent) sendm) as fromM'.
+      pose proof (cRecvRespPrevState pDef nDef p_parent recvm sendm) as same.
       rewrite <- fromM' in same.
       rewrite <- same in fromM.
       rewrite fromM in easy.
       unfold sle in easy; firstorder.
-      destruct toChild as [c' [c'_child _]].
+      destruct toChild as [c' [c'Def [c'_child _]]].
       unfold parent in c'_child; firstorder.
       destruct deqSt as [l [i deqSt]].
-      pose proof (deqImpData deqSt) as newData.
+      pose proof (deqImpData nDef deqSt) as newData.
       rewrite newData.
       assert (e1: t < S t) by omega.
-      assert (e2: forall ti, t < ti < S t -> forall ci li ii, ~ deqR ci li a St ii ti) by
+      assert (e2: forall ti, t < ti < S t -> forall ci li ii, defined ci ->
+                                                              ~ deqR ci li a St ii ti) by
           (intros ti [cond1 cond2]; assert (f: False) by omega; firstorder).
-      generalize e1 e2 deqSt; clear; firstorder.
+      generalize e1 e2 nDef deqSt; clear; firstorder.
       assert (inv: state (Child n) a t = In) by
           (unfold sle in hard; destruct (state (Child n) a t); firstorder).
       clear hard.
@@ -444,8 +463,8 @@ Module LatestValueTheorems (dt: DataTypes) (ch: ChannelPerAddr dt) (c: BehaviorA
       pose proof (slt_neq' upgrade) as neq'.
       assert (neq: state (Child n) a (S t) <> state (Child n) a t) by auto.
       assert (c_child: parent (Child n) Parent) by (unfold parent; auto).
-      pose proof (change (st c_child) neq) as [[m markm] | [m recvm]].
-      pose proof (cSendDowngrade c_child markm) as dwn.
+      pose proof (change (st defParent nDef c_child) neq) as [[m markm] | [m recvm]].
+      pose proof (cSendDowngrade defParent nDef c_child markm) as dwn.
       pose proof (slt_slti_false upgrade dwn) as f.
       firstorder.
       pose proof (recvImpMark recvm) as [ts [ts_le_t sendm]].
@@ -457,20 +476,20 @@ Module LatestValueTheorems (dt: DataTypes) (ch: ChannelPerAddr dt) (c: BehaviorA
       pose proof @pSendPSameState as mui2.
 
 
-      pose proof (sendmFrom (dt c_child) sendm) as fromY.
-      pose proof (sendmChange (dt c_child) sendm) as toT.
-      pose proof (pSendUpgrade c_child sendm) as upd.
+      pose proof (sendmFrom (dt defParent nDef c_child) sendm) as fromY.
+      pose proof (sendmChange (dt defParent nDef c_child) sendm) as toT.
+      pose proof (pSendUpgrade defParent nDef c_child sendm) as upd.
 
       assert (pHigh: forall tx, ts < tx < S t -> slt In (dir Parent c a tx)).
       intros tx cond. assert (cond2: ts < tx <= t) by omega.
-      pose proof (pSendPSameState c_child sendm recvm cond2) as sth.
+      pose proof (pSendPSameState defParent nDef c_child sendm recvm cond2) as sth.
       rewrite <- toT in sth.
       rewrite <- sth in upd.
       unfold slt in *; destruct (dir Parent c a ts); destruct (dir Parent c a tx); auto.
       assert (cLow: forall tx, ts < tx < S t -> slt (state c a tx) Mo).
       intros tx cond. assert (cond2: ts <= tx <= t) by omega.
-      pose proof (pSendCSameState c_child sendm recvm cond2) as sth.
-      pose proof (conservative c_child a ts) as cons11.
+      pose proof (pSendCSameState defParent nDef c_child sendm recvm cond2) as sth.
+      pose proof (conservative defParent nDef c_child a ts) as cons11.
       rewrite <- sth in cons11.
       unfold slt in *; unfold sle in *; destruct (state c a tx); destruct (dir Parent c a ts);
       destruct (dir Parent c a (S ts)); auto.
@@ -479,77 +498,79 @@ Module LatestValueTheorems (dt: DataTypes) (ch: ChannelPerAddr dt) (c: BehaviorA
 
 
       assert (others: forall tx, ts < tx < S t ->
-                                 forall c', c' <> c -> parent c' Parent ->
+                                 forall c', defined c' -> c' <> c -> parent c' Parent ->
                                             sle (dir Parent c' a tx)
                                                 match dir Parent c a tx with
                                                   | In => Mo
                                                   | Sh => Sh
                                                   | Mo => In
                                                 end) by
-          (intros tx _; apply (compatible a tx c_child)).
+          (intros tx _; apply (compatible defParent a tx nDef c_child)).
       assert (c'DirLow:
                 forall tx,
                   ts < tx < S t -> 
-                  forall c', c' <> c -> parent c' Parent -> slt (dir Parent c' a tx) Mo).
-      intros tx cond c' c'_ne_c c'_child.
-      specialize (others tx cond c' c'_ne_c c'_child).
+                  forall c', defined c' ->
+                             c' <> c -> parent c' Parent -> slt (dir Parent c' a tx) Mo).
+      intros tx cond c' c'Def c'_ne_c c'_child.
+      specialize (others tx cond c' c'Def c'_ne_c c'_child).
       specialize (pHigh tx cond).
       unfold slt in *; destruct (dir Parent c a tx); destruct (dir Parent c' a tx); auto.
-      assert (c'Low: forall tx, ts < tx < S t -> forall c',
+      assert (c'Low: forall tx, ts < tx < S t -> forall c', defined c' ->
                                                    c' <> c ->
                                                    parent c' Parent ->
                                                    slt (state c' a tx) Mo).
-      intros tx cond c' c'_ne_c c'_child.
-      specialize (c'DirLow tx cond c' c'_ne_c c'_child).
-      pose proof (conservative c'_child a tx) as sig.
+      intros tx cond c' c'Def c'_ne_c c'_child.
+      specialize (c'DirLow tx cond c' c'Def c'_ne_c c'_child).
+      pose proof (conservative defParent c'Def c'_child a tx) as sig.
       unfold slt in *; destruct (dir Parent c' a tx); destruct (state c' a tx); auto.
-      assert (allLow: forall tx, ts < tx < S t -> forall c0,
+      assert (allLow: forall tx, ts < tx < S t -> forall c0, defined c0 ->
                                            parent c0 Parent -> slt (state c0 a tx) Mo).
-      intros tx cond c0 c0_child.
+      intros tx cond c0 c0Def c0_child.
       assert (cache: {c0 = c} + {c0 <> c}) by (
                                         decide equality;
                                         decide equality).
       destruct cache as [eq|notEq].
       rewrite eq in *; apply (cLow tx cond).
-      apply (c'Low tx cond c0 notEq c0_child).
+      apply (c'Low tx cond c0 c0Def notEq c0_child).
       assert (noSt: forall ti, ts < ti < S t ->
-                               forall ci li ii, ~ deqR ci li a St ii ti).
-      unfold not; intros ti cond ci li ii deqSt.
+                               forall ci li ii, defined ci -> ~ deqR ci li a St ii ti).
+      unfold not; intros ti cond ci li ii ciDef deqSt.
       pose proof (deqLeaf deqSt) as leafCi.
       assert(ci_child: parent ci Parent) by (unfold leaf in *; unfold parent in *; auto).
       pose proof (processDeq deqSt) as mustMo.
       simpl in *.
-      specialize (allLow ti cond ci ci_child).
+      specialize (allLow ti cond ci ciDef ci_child).
       unfold sle in allLow; destruct (state ci a ti); auto; discriminate.
 
       
-      pose proof (cRecvRespPrevState c_child recvm sendm) as prevState.
-      pose proof (sendmFrom (dt c_child) sendm) as fromM.
+      pose proof (cRecvRespPrevState defParent nDef c_child recvm sendm) as prevState.
+      pose proof (sendmFrom (dt defParent nDef c_child) sendm) as fromM.
       rewrite <- fromM in prevState.
       rewrite prevState in inv.
-      pose proof (fromParent c_child recvm inv) as dM.
-      pose proof (toChild c_child sendm inv) as dM'.
+      pose proof (fromParent nDef defParent c_child recvm inv) as dM.
+      pose proof (toChild nDef defParent c_child sendm inv) as dM'.
       rewrite dM' in dM; rewrite dM.
       assert (le: ts <= t) by omega.
       assert (stCond: sle Sh (state Parent a ts)) by
           (
            specialize (stEq ts); rewrite stEq; unfold sle; auto).
-      pose proof (sendCCond c_child sendm) as [_ rest].
-      pose proof (recvmChange (st c_child) recvm) as newState.
+      pose proof (sendCCond defParent nDef c_child sendm) as [_ rest].
+      pose proof (recvmChange (st defParent nDef c_child) recvm) as newState.
       rewrite <- newState in rest.
-      assert (cond1: forall c0, c0 <> c -> parent c0 Parent -> sle (dir Parent c0 a ts) Sh) by
+      assert (cond1: forall c0, defined c0 ->
+                                c0 <> c -> parent c0 Parent -> sle (dir Parent c0 a ts) Sh) by
           (
-          intros c0 cond c0_child; specialize (rest c0 cond c0_child);
+          intros c0 c0Def cond c0_child; specialize (rest c0 c0Def cond c0_child);
           destruct (state c a (S t)); destruct (dir Parent c0 a ts);
           unfold sle in *; unfold slt in *; auto).
       rewrite inv in fromM.
-      assert (cond2: forall c, parent c Parent -> sle (dir Parent c a ts) Sh).
-          intros c0 c0_child; assert (H2: {c0 = c} + {c0 <> c}) by 
+      assert (cond2: forall c, defined c -> parent c Parent -> sle (dir Parent c a ts) Sh).
+          intros c0 c0Def c0_child; assert (H2: {c0 = c} + {c0 <> c}) by 
                                  (decide equality; decide equality);
           destruct H2 as [easy | hard].
           rewrite easy in *; rewrite <- fromM; unfold sle; auto.
-          apply (cond1 c0 hard c0_child).
-      pose proof (SIHt ts le Parent (conj stCond cond2)) as useful.
+          apply (cond1 c0 c0Def hard c0_child).
+      pose proof (SIHt ts le Parent defParent (conj stCond cond2)) as useful.
       destruct (data Parent a ts).
       intros ti condx.
       assert (cond3: 0 <= ti < ts \/ ts < ti < S t \/ ti = ts) by omega.
@@ -557,38 +578,39 @@ Module LatestValueTheorems (dt: DataTypes) (ch: ChannelPerAddr dt) (c: BehaviorA
       generalize noSt e1 useful; clear; firstorder.
       generalize noSt e2 useful; clear; firstorder.
       rewrite e3 in *.
-      pose proof (sendCCond c_child sendm) as [_ use].
-      pose proof (pSendUpgrade c_child sendm) as upg.
-      pose proof (sendmChange (dt c_child) sendm) as upg2.
+      pose proof (sendCCond defParent nDef c_child sendm) as [_ use].
+      pose proof (pSendUpgrade defParent nDef c_child sendm) as upg.
+      pose proof (sendmChange (dt defParent nDef c_child) sendm) as upg2.
       rewrite <- fromM in upg; rewrite upg2 in upg.
-      assert (othersNot: forall c', c' <> c -> parent c' Parent ->
+      assert (othersNot: forall c', defined c' -> c' <> c -> parent c' Parent ->
                                     dir Parent c' a ts <> Mo).
-      intros c' c'_ne c'_child.
-      specialize (use c' c'_ne c'_child).
+      intros c' c'Def c'_ne c'_child.
+      specialize (use c' c'Def c'_ne c'_child).
       destruct (dir Parent c' a ts); destruct (to m); unfold slt in *; unfold sle in *; auto;
       discriminate.
-      assert (allNot: forall c', parent c' Parent ->
+      assert (allNot: forall c', defined c' -> parent c' Parent ->
                                  dir Parent c' a ts <> Mo).
       intros c'.
       assert (eqOrNot: {c' = c} + {c' <> c}) by (decide equality; decide equality).
       destruct eqOrNot as [eq|not].
       rewrite eq in *; rewrite <- fromM; intros; discriminate.
       generalize othersNot not; clear; firstorder.
-      assert (allNot': forall c', parent c' Parent -> state c' a ts <> Mo).
-      intros c' parentc'. specialize (allNot c' parentc').
-      pose proof (conservative parentc' a ts) as slee.
+      assert (allNot': forall c', defined c' -> parent c' Parent -> state c' a ts <> Mo).
+      intros c' c'Def parentc'. specialize (allNot c' c'Def parentc').
+      pose proof (conservative defParent c'Def parentc' a ts) as slee.
       unfold sle in *; destruct (state c' a ts); destruct (dir Parent c' a ts);
       auto; discriminate.
-      unfold not; intros.
+      unfold not; intros ci li ii ciDef. intros.
       pose proof (deqLeaf H0) as leafc.
       pose proof (processDeq H0) as procc.
       simpl in *.
       assert (parent ci Parent) by (unfold parent; destruct ci; auto).
-      generalize allNot' procc H1; clear; firstorder.
+      generalize allNot' ciDef procc H1; clear; firstorder.
 
 
-      destruct useful as [cb [ib [tb [tbTs [deqTb rest2]]]]].
+      destruct useful as [cb [ib [tb [cbDef [tbTs [deqTb rest2]]]]]].
       exists cb; exists ib; exists tb.
+      constructor. assumption.
       assert (tsLeSt: ts <= S t) by omega.
       constructor. 
       assert (tb < S t) by omega.
@@ -600,54 +622,57 @@ Module LatestValueTheorems (dt: DataTypes) (ch: ChannelPerAddr dt) (c: BehaviorA
       generalize noSt e1 rest2; clear; firstorder.
       generalize noSt e2 rest2; clear; firstorder.
       rewrite e3 in *.
-      pose proof (sendCCond c_child sendm) as [_ use].
-      pose proof (pSendUpgrade c_child sendm) as upg.
-      pose proof (sendmChange (dt c_child) sendm) as upg2.
+      pose proof (sendCCond defParent nDef c_child sendm) as [_ use].
+      pose proof (pSendUpgrade defParent nDef c_child sendm) as upg.
+      pose proof (sendmChange (dt defParent nDef c_child) sendm) as upg2.
       rewrite <- fromM in upg; rewrite upg2 in upg.
-      assert (othersNot: forall c', c' <> c -> parent c' Parent ->
+      assert (othersNot: forall c', defined c' -> c' <> c -> parent c' Parent ->
                                     dir Parent c' a ts <> Mo).
-      intros c' c'_ne c'_child.
-      specialize (use c' c'_ne c'_child).
+      intros c' c'Def c'_ne c'_child.
+      specialize (use c' c'Def c'_ne c'_child).
       destruct (dir Parent c' a ts); destruct (to m); unfold slt in *; unfold sle in *; auto;
       discriminate.
-      assert (allNot: forall c', parent c' Parent ->
+      assert (allNot: forall c', defined c' -> parent c' Parent ->
                                  dir Parent c' a ts <> Mo).
       intros c'.
       assert (eqOrNot: {c' = c} + {c' <> c}) by (decide equality; decide equality).
       destruct eqOrNot as [eq|not].
       rewrite eq in *; rewrite <- fromM; intros; discriminate.
       generalize othersNot not; clear; firstorder.
-      assert (allNot': forall c', parent c' Parent -> state c' a ts <> Mo).
-      intros c' parentc'. specialize (allNot c' parentc').
-      pose proof (conservative parentc' a ts) as slee.
+      assert (allNot': forall c', defined c' -> parent c' Parent -> state c' a ts <> Mo).
+      intros c' c'Def parentc'. specialize (allNot c' c'Def parentc').
+      pose proof (conservative defParent c'Def parentc' a ts) as slee.
       unfold sle in *; destruct (state c' a ts); destruct (dir Parent c' a ts);
       auto; discriminate.
-      unfold not; intros.
+      unfold not; intros ci li ii ciDef. intros.
       pose proof (deqLeaf H0) as leafc.
       pose proof (processDeq H0) as procc.
       simpl in *.
       assert (parent ci Parent) by (unfold parent; destruct ci; auto).
-      generalize allNot' procc H1; clear; firstorder.
+      generalize allNot' procc ciDef H1; clear; firstorder.
     Qed.
 
   End ForAddr.
 
   Theorem latestValue:
-  forall {c a t},
+  forall {c a t}, defined c ->
     leaf c ->
     sle Sh (state c a t) ->
     match data c a t with
-      | Initial => forall {ti}, 0 <= ti < t -> forall {ci li ii}, ~ deqR ci li a St ii ti
+      | Initial => forall {ti}, 0 <= ti < t -> forall {ci li ii}, 
+                                                 defined ci -> ~ deqR ci li a St ii ti
       | Store lb =>
-        exists cb ib tb, tb < t /\ deqR cb lb a St ib tb /\
-                         forall {ti}, tb < ti < t -> forall {ci li ii}, ~ deqR ci li a St ii ti
+        exists cb ib tb, defined cb /\ tb < t /\ deqR cb lb a St ib tb /\
+                         forall {ti}, tb < ti < t -> forall {ci li ii},
+                                                       defined ci -> ~ deqR ci li a St ii ti
     end.
   Proof.
-    intros c a t leafC more.
-    assert (sth: forall c', parent c' c -> sle (dir c c' a t) Sh) by
-        ( intros c' c'_child; unfold parent in *; unfold leaf in *; destruct c; destruct c';
+    intros c a t cDef leafC more.
+    assert (sth: forall c', defined c' -> parent c' c -> sle (dir c c' a t) Sh) by
+        ( intros c' c'Def c'_child; unfold parent in *; unfold leaf in *;
+                                    destruct c; destruct c';
           firstorder).
-    pose proof (allLatestValue (conj more sth)) as useful.
+    pose proof (allLatestValue cDef (conj more sth)) as useful.
     assumption.
   Qed.
 
